More progress in Propositional Logic.

PropositionalLogic/Semantics/Trivial.v
@@ -1,5 +1,6 @@
 Require Import Logic.GeneralLogic.Base.
 Require Import Logic.MinimunLogic.Syntax.
+Require Import Logic.MinimunLogic.Semantics.Trivial.
 Require Import Logic.PropositionalLogic.Syntax.
 
 Local Open Scope logic_base.
@@ -7,9 +8,6 @@ Local Open Scope syntax.
 Import PropositionalLanguageNotation.
 
 Module Semantics.
-
-Definition impp {model: Type} (X: Ensemble model) (Y: Ensemble model): Ensemble model :=
-  fun m => X m -> Y m.
 
 Definition andp {model: Type} (X: Ensemble model) (Y: Ensemble model): Ensemble model :=
   fun m => X m /\ Y m.
@@ -21,22 +19,22 @@ Definition falsep {model: Type}: Ensemble model := fun m => False.
 
 End Semantics.
 
-Class TrivialPropositionalSemantics (L: Language) {nL: NormalLanguage L} {pL: PropositionalLanguage L} (MD: Model) (SM: Semantics L MD): Type := {
-  denote_impp: forall x y, Same_set _ (denotation (x --> y)) (Semantics.impp (denotation x) (denotation y));
+Class TrivialPropositionalSemantics (L: Language) {minL: MinimunLanguage L} {pL: PropositionalLanguage L} (MD: Model) (SM: Semantics L MD): Type := {
   denote_andp: forall x y, Same_set _ (denotation (x && y)) (Semantics.andp (denotation x) (denotation y));
   denote_orp: forall x y, Same_set _ (denotation (x || y)) (Semantics.orp (denotation x) (denotation y));
   denote_falsep: Same_set _ (denotation FF) Semantics.falsep
 }.
 
-Lemma sat_impp {L: Language} {nL: NormalLanguage L} {pL: PropositionalLanguage L} {MD: Model} {SM: Semantics L MD} {tpSM: TrivialPropositionalSemantics L MD SM}: forall m x y, m |= x --> y <-> (m |= x -> m |= y).
-Proof.
-  intros; simpl.
-  unfold satisfies.
-  destruct (denote_impp x y).
-  split; auto; [apply H | apply H0].
-Qed.
+Section Trivial.
 
-Lemma sat_andp {L: Language} {nL: NormalLanguage L} {pL: PropositionalLanguage L} {MD: Model} {SM: Semantics L MD} {tpSM: TrivialPropositionalSemantics L MD SM}: forall m x y, m |= x && y <-> (m |= x /\ m |= y).
+Context {L: Language}
+        {minL: MinimunLanguage L}
+        {pL: PropositionalLanguage L}
+        {MD: Model}
+        {SM: Semantics L MD}
+        {tpSM: TrivialPropositionalSemantics L MD SM}.
+
+Lemma sat_andp: forall m x y, m |= x && y <-> (m |= x /\ m |= y).
 Proof.
   intros; simpl.
   unfold satisfies.
@@ -44,7 +42,7 @@ Proof.
   split; auto; [apply H | apply H0].
 Qed.
 
-Lemma sat_orp {L: Language} {nL: NormalLanguage L} {pL: PropositionalLanguage L} {MD: Model} {SM: Semantics L MD} {tpSM: TrivialPropositionalSemantics L MD SM}: forall m x y, m |= x || y <-> (m |= x \/ m |= y).
+Lemma sat_orp: forall m x y, m |= x || y <-> (m |= x \/ m |= y).
 Proof.
   intros; simpl.
   unfold satisfies.
@@ -52,10 +50,12 @@ Proof.
   split; auto; [apply H | apply H0].
 Qed.
 
-Lemma sat_falsep {L: Language} {nL: NormalLanguage L} {pL: PropositionalLanguage L} {MD: Model} {SM: Semantics L MD} {tpSM: TrivialPropositionalSemantics L MD SM}: forall m, m |= FF <-> False.
+Lemma sat_falsep: forall m, m |= FF <-> False.
 Proof.
   intros; simpl.
   unfold satisfies.
   destruct denote_falsep.
   split; auto; [apply H | apply H0].
 Qed.
+
+End Trivial.
